add IsRen and remove autoimpl

LeanSubst/Map.lean
@@ -1,21 +1,24 @@
 import LeanSubst.Basic
 
 namespace LeanSubst
+  section
+    universe u v
+    variable {A : Type u} {B : Type v} {f : A -> B}
 
     @[simp]
-    def map (f : A -> B) : Subst A -> Subst B
+    def map {A B} (f : A -> B) : Subst A -> Subst B
     | σ, n =>
       match (σ n) with
       | .su t => .su (f t)
       | .re k => .re k
 
     @[simp]
-    theorem map_rename_seq : map f (.re k :: σ) = .re k :: map f σ := by
+    theorem map_rename_seq {k} {σ : Subst A} : map f (.re k :: σ) = .re k :: map f σ := by
       funext; case _ x =>
       cases x <;> simp
 
     @[simp]
-    theorem map_replace_seq : map f (.su t :: σ) = .su (f t) :: map f σ := by
+    theorem map_replace_seq {t} {σ : Subst A} : map f (.su t :: σ) = .su (f t) :: map f σ := by
       funext; case _ x =>
       cases x <;> simp
 
@@ -31,7 +34,7 @@ namespace LeanSubst
     @[simp]
     theorem map_S_noop : map f S = S := by apply map_rename_noop
 
-    theorem map_rename_compose_left {A B} {τ : Subst A} [SubstMap A] [SubstMap B] {f : A -> B} {r : Ren}
+    theorem map_rename_compose_left {τ : Subst A} [SubstMap A] [SubstMap B] {f : A -> B} {r : Ren}
       : (∀ t, f (t[r.to]) = (f t)[r.to]) -> map f (τ ∘ r.to) = (map f τ) ∘ r.to
     := by
       intro h
@@ -43,21 +46,22 @@ namespace LeanSubst
       case _ t => apply h
 
     @[simp]
-    theorem map_rename_compose_right {A B} {σ : Subst A} [SubstMap A] [SubstMap B] {f : A -> B} {r : Ren}
+    theorem map_rename_compose_right {σ : Subst A} [SubstMap A] [SubstMap B] {f : A -> B} {r : Ren}
       : map f (r.to ∘ σ) = r.to ∘ (map f σ)
     := by
       unfold Subst.compose; simp
       funext; case _ x =>
         unfold Ren.to; simp
 
-    theorem map_S_compose_left {A B} {τ : Subst A} [SubstMap A] [SubstMap B] {f : A -> B}
+    theorem map_S_compose_left {τ : Subst A} [SubstMap A] [SubstMap B] {f : A -> B}
       : (∀ t, f (t[S]) = (f t)[S]) -> map f (τ ∘ S) = (map f τ) ∘ S
     := by
       intro h
       apply map_rename_compose_left h
 
     @[simp]
-    theorem map_S_compose_right {A B} {σ : Subst A} [SubstMap A] [SubstMap B] {f : A -> B}
+    theorem map_S_compose_right {σ : Subst A} [SubstMap A] [SubstMap B] {f : A -> B}
       : map f (S ∘ σ) = S ∘ (map f σ)
     := by apply map_rename_compose_right
+  end
 end LeanSubst
